examples/mw/MWAll.v
@@ -1,0 +1,248 @@
+Require Import Coqlib ITreelib ImpPrelude STS Behavior.
+Require Import ModSem Skeleton PCM STB Open OpenDef Hoare HoareDef Imp.
+Require Import Mem0 Mem1 MemOpen Mem0Openproof MemOpen0proof.
+Require Import
+        MWHeader
+        MWCImp MWC9 MWC0 MWC1 MWC2 MWCImp9proof MWC90proof MWC01proof MWC12proof
+        MWApp0 MWApp1 MWApp2 MWApp01proof MWApp12proof
+.
+
+Set Implicit Arguments.
+
+
+
+Definition MWGRA: GRA.t := GRA.of_list [Mem1.memRA; spRA; mapRA; mwRA; AppRA.t].
+Local Existing Instance MWGRA.
+
+Instance memRA_inG: @GRA.inG Mem1.memRA MWGRA.
+Proof. exists 0. ss. Defined.
+Local Existing Instance memRA_inG.
+
+Instance spRA_inG: @GRA.inG spRA MWGRA.
+Proof. exists 1. ss. Defined.
+Local Existing Instance spRA_inG.
+
+Instance mapRA_inG: @GRA.inG mapRA MWGRA.
+Proof. exists 2. ss. Defined.
+Local Existing Instance mapRA_inG.
+
+Instance mwRA_inG: @GRA.inG mwRA MWGRA.
+Proof. exists 3. ss. Defined.
+Local Existing Instance mwRA_inG.
+
+Instance AppRA_inG: @GRA.inG AppRA.t MWGRA.
+Proof. exists 4. ss. Defined.
+Local Existing Instance AppRA_inG.
+
+Section PROOF.
+
+(*   Check (to_stb_context ["new"; "access"; "update"; "init"; "run"] (MWStb ++ MemStb)). *)
+(*   Check (@to_closed_stb MWGRA ∘ @KMod.get_stb MWGRA [@KMem MWGRA memRA_inG; @KMW MWGRA memRA_inG]). *)
+  Let abc_correct :
+∀ (Σ : GRA.t) (H : GRA.inG memRA Σ) (global_stb : Sk.t -> string → option HoareDef.fspec),
+  (forall sk, stb_incl (to_stb_context ["new"; "access"; "update"; "init"; "run"] (MemStb)) (global_stb sk))
+  → refines2 [MWCImp.MW] [MWC9.MW (global_stb)].
+  admit "".
+  Qed.
+
+  Let MWLow: refines2 [Mem0.Mem; MWCImp.MW] [Mem0.Mem; MWC0.MW].
+  Proof.
+    transitivity (KMod.transl_tgt_list [KMem; MWC9.KMW]).
+    { eapply refines2_cons.
+      { eapply Mem0Openproof.correct. }
+      { eapply abc_correct. i.
+        eapply to_stb_context_incl.
+        { etrans.
+          { eapply incl_appl; refl. }
+          cbn. unfold MemStb. autounfold with stb. autorewrite with stb. cbn. refl.
+        }
+        ImpProofs.solve_NoDup.
+      }
+    }
+    etrans.
+    { eapply adequacy_open. i. exists ε. split.
+      { g_wf_tac.
+        Local Transparent Sk.load_skenv _points_to string_dec.
+        unfold var_points_to.
+        rewrite URA.unit_idl.
+        ur. unfold var_points_to, initial_mem_mr. ss. uo. idtac. split.
+        2: { ur. i. ur. i. ur. des_ifs. }
+        { repeat rewrite URA.unit_id. ur. eexists ε.
+          repeat rewrite URA.unit_id. extensionality k. extensionality n.
+          unfold sumbool_to_bool, andb. des_ifs.
+          { ss. clarify. }
+          { ss. clarify. exfalso. lia. }
+          { repeat (destruct k; ss). }
+        }
+      }
+
+      { g_wf_tac. repeat (i; splits; ur; ss). refl. }
+      { ii. ss. }
+    }
+
+    
+          eapply incl_appl.
+        cbn. rr. unfold to_stb_context, to_stb. ii. ss. stb_tac.
+        des_ifs.
+        apply_all_once rel_dec_correct. subst.
+        Local Transparent
+        unfold rel_dec in *. des_ifs.
+        unfold to_stb_context. unfold to_closed_stb. ss.
+        etrans; [|eapply to_closed_stb_weaker]. stb_incl_tac; try tauto. }
+        i. ss. refl. }
+      eapply MWCImp9proof.correct.
+      etrans.
+      { eapply MWCImp9proof.correct. refl. }
+      { unfold MWC9.MW. Set Printing Implicit. Unset Printing Notations. Set Printing All. unfold KMW.
+        (@to_closed_stb MWGRA ∘ @KMod.get_stb MWGRA [@KMem MWGRA memRA_inG; @KMW MWGRA memRA_inG])
+        TTTTTTTTTTTTTTT
+        eapply MWC90proof.correct.
+
+      
+      eapply refines2_cons; [|refl].
+      { etrans.
+        { eapply StackImp0proof.correct. }
+        { eapply Stack01proof.correct. i.
+          etrans; [|eapply to_closed_stb_weaker]. stb_incl_tac; tauto. }
+      }
+    }
+
+    {
+    }
+    etrans.
+    { eapply adequacy_open. i. exists ε. split.
+      { g_wf_tac. repeat (i; splits; ur; ss). refl. }
+      { ii. ss. }
+
+    }
+  Qed.
+
+  Theorem mw_correct:
+    refines2 [Mem0.Mem; MWCImp.MW.Stack; EchoImp.Echo]
+             [Mem0.Mem; Stack2.Stack; KMod.transl_src (fun _ => ["Echo"]) KEcho].
+  Proof.
+  Qed.
+End PROOF.
+
+
+
+(* Imp program *)
+Require Import Mem0 StackImp EchoImp EchoMainImp ClientImp.
+Section ECHOIMP.
+  Definition echo_progs := [Stack_prog; Echo_prog; EchoMain_prog; Client_prog].
+  Definition echo_imp: ModL.t :=
+    Mod.add_list (Mem :: map ImpMod.get_mod echo_progs).
+
+  Definition echo_imp_itr := ModSemL.initial_itr (ModL.enclose echo_imp) None.
+End ECHOIMP.
+
+
+Require Import Mem0 Stack0 Echo0 EchoMain0 Client0.
+Section ECHOIMPL.
+  Definition echo_impl: ModL.t :=
+    Mod.add_list [Mem; Stack; Echo; Main; Client].
+
+  Definition echo_impl_itr := ModSemL.initial_itr (ModL.enclose echo_impl) None.
+End ECHOIMPL.
+
+
+Require Import MemOpen Stack3A Echo1 EchoMain0 Client0.
+(* spec program *)
+Require Import Stack2.
+Section ECHOSPEC.
+  Definition echo_spec: ModL.t :=
+    Mod.add_list [
+        Mem0.Mem;
+      Stack2.Stack;
+      KMod.transl_src (fun _ => ["Echo"]) KEcho;
+      Main; Client
+      ].
+
+  Definition echo_spec_itr := ModSemL.initial_itr (ModL.enclose echo_spec) None.
+End ECHOSPEC.
+
+
+
+Require Import Mem0Openproof MemOpen0proof.
+Require Import StackImp0proof Stack01proof Stack12proof Stack23Aproof.
+Require Import EchoMainImp0proof EchoImp0proof.
+Require Import ClientImp0proof Echo01proof.
+Require Import Echo1mon Stack32proof.
+Section PROOF.
+  Theorem echo_correct:
+    refines2 [Mem0.Mem; StackImp.Stack; EchoImp.Echo]
+             [Mem0.Mem; Stack2.Stack; KMod.transl_src (fun _ => ["Echo"]) KEcho].
+  Proof.
+    transitivity (KMod.transl_tgt_list [KMem; Stack1.KStack]++[EchoImp.Echo]).
+    { eapply refines2_cons.
+      { eapply Mem0Openproof.correct. }
+      eapply refines2_cons; [|refl].
+      { etrans.
+        { eapply StackImp0proof.correct. }
+        { eapply Stack01proof.correct. i.
+          etrans; [|eapply to_closed_stb_weaker]. stb_incl_tac; tauto. }
+      }
+    }
+    etrans.
+    { eapply refines2_app; [|refl].
+      eapply adequacy_open. i. exists ε. split.
+      { g_wf_tac. repeat (i; splits; ur; ss). refl. }
+      { ii. ss. }
+    }
+    eapply refines2_cons.
+    { eapply MemOpen0proof.correct. }
+    transitivity (KMod.transl_tgt_list [Stack3A.KStack; KEcho]).
+    { eapply refines2_cons.
+      { etrans.
+        { eapply Stack12proof.correct. }
+        { eapply Stack23Aproof.correct. }
+      }
+      { etrans.
+        { eapply EchoImp0proof.correct. }
+        { eapply Echo01proof.correct.
+          stb_context_incl_tac; tauto. }
+      }
+    }
+    etrans.
+    { eapply adequacy_open. i. exists ε. split.
+      { g_wf_tac; repeat (i; splits; ur; ss). refl. }
+      { ii. ss. }
+    }
+    { eapply refines2_cons.
+      { eapply Stack32proof.correct. }
+      eapply refines2_cons; [|refl].
+      { eapply Echo1mon.correct. ii. ss. des; auto. }
+    }
+  Qed.
+
+  Corollary echo_closed_correct:
+    refines_closed echo_imp echo_spec.
+  Proof.
+    eapply refines_close. hexploit refines2_app.
+    { eapply echo_correct. }
+    { eapply refines2_cons.
+      { eapply EchoMainImp0proof.correct. }
+      { eapply ClientImp0proof.correct. }
+    }
+    ss.
+  Qed.
+End PROOF.
+
+
+Require Import SimSTS2 Imp2Csharpminor Imp2Asm.
+Require Import Imp2AsmProof.
+Section PROOF.
+  Context `{builtins : builtinsTy}.
+  Hypothesis source_linking: exists impl, link_imps echo_progs = Some impl.
+
+  Theorem echo_compile_correct
+          (asms : Coqlib.nlist Asm.program)
+          (COMP: Forall2 (fun imp asm => compile_imp imp = Errors.OK asm) echo_progs asms)
+    :
+      exists asml, (Linking.link_list asms = Some asml) /\
+                   (improves2_program (ModL.compile echo_spec) (Asm.semantics asml)).
+  Proof.
+    hexploit compile_behavior_improves; [et|et|]. i. des. esplits; [et|].
+    eapply improves_combine; [|et]. eapply echo_closed_correct.
+  Qed.
+End PROOF.
