examples/mw/MWApp9.v
@@ -1,0 +1,85 @@
+Require Import Coqlib.
+Require Import ITreelib.
+Require Import ImpPrelude.
+Require Import STS.
+Require Import Behavior.
+Require Import ModSem.
+Require Import Skeleton.
+Require Import MWHeader.
+Require Import PCM.
+Require Import HoareDef OpenDef STB.
+Require Import Mem1.
+
+Set Implicit Arguments.
+
+
+
+Section PROOF.
+
+  (* Definition pget A: itree Es A := (p0 <- trigger PGet;; `p0: A <- p0↓ǃ;; Ret p0). *)
+  (* Definition pput A (p0: A) := (trigger (PPut p0↑)). *)
+  Notation pget := (p0 <- trigger PGet;; p0 <- p0↓ǃ;; Ret p0) (only parsing).
+  Notation pput p0 := (trigger (PPut p0↑)) (only parsing).
+
+  Notation check_lock := (p0 <- trigger PGet;; if (Any.split p0) then triggerUB else Ret tt) (only parsing).
+  Notation lAPC := (p0 <- trigger PGet;; _ <- trigger (PPut (Any.pair tt↑ p0));;; trigger (PPut p0))
+                     (only parsing).
+
+  Let Es := (hAPCE +' Es).
+
+  Definition initF: list val -> itree Es val :=
+    fun varg =>
+      _ <- (pargs [] varg)?;;
+      check_lock;;;
+      lAPC;;;
+      initialized <- pget;;
+      if (initialized: bool)
+      then syscallU "print" [(- 1)%Z];;; Ret Vundef
+      else `_: val <- ccallU "put" [Vint 0; Vint 42];; pput true;;; Ret Vundef
+  .
+
+  Definition runF: list val -> itree Es val :=
+    fun varg =>
+      _ <- (pargs [] varg)?;;
+      check_lock;;;
+      lAPC;;;
+      initialized <- pget;;
+      if negb (initialized: bool)
+      then syscallU "print" [(- 1)%Z];;; Ret Vundef
+      else `v: val <- ccallU "get" [Vint 0];; v <- (pargs [Tint] [v])?;; syscallU "print" [v];;; Ret Vundef
+  .
+
+  Context `{Σ: GRA.t}.
+  Context `{@GRA.inG memRA Σ}.
+
+  Definition Appsbtb: list (string * kspecbody) :=
+    [("init", ksb_trivial (cfunU initF)); ("run", ksb_trivial (cfunU runF))].
+
+  Definition AppStb: list (gname * fspec).
+    eapply (Seal.sealing "stb").
+    let x := constr:(List.map (map_snd (fun ksb => ksb.(ksb_fspec): fspec)) Appsbtb) in
+    let y := eval cbn in x in
+    eapply y.
+  Defined.
+
+  Definition KAppSem ske: KModSem.t := {|
+    KModSem.fnsems := Appsbtb;
+    KModSem.mn := "App";
+    KModSem.initial_mr := GRA.embed (var_points_to ske "initialized" (Vint 0)) ;
+    KModSem.initial_st := false↑;
+  |}
+  .
+
+  (* Definition MWSem (stb: gname -> option fspec): ModSem.t := *)
+  (*   KModSem.transl_tgt stb KMWSem. *)
+
+  Definition KApp: KMod.t := {|
+    KMod.get_modsem := fun sk => KAppSem (Sk.load_skenv sk);
+    KMod.sk := []
+  |}
+  .
+
+  Definition App (stb: Sk.t -> gname -> option fspec): Mod.t := (KMod.transl_tgt stb KApp).
+
+End PROOF.
+Global Hint Unfold AppStb: stb.
